\documentclass[reqno]{amsart}
\usepackage{amscd, amssymb, amsmath, amsthm}
\usepackage{graphicx}
\usepackage[colorlinks=true,linkcolor=blue]{hyperref}
\usepackage[utf8]{inputenc}
\usepackage[T1]{fontenc}
\usepackage{textcomp}
\usepackage{babel}
%% for identity function 1:
\usepackage{bbm}
%%For category theory diagrams:
\usepackage{tikz-cd}

%\usepackage[backend=biber]{biblatex}
%\addbibresource{.bib}


\setlength\parindent{0pt}
\pdfsuppresswarningpagegroup=1



\newtheorem{theorem}{Theorem}[section]
\newtheorem{lemma}[theorem]{Lemma}
\newtheorem{proposition}[theorem]{Proposition}
\newtheorem{corollary}[theorem]{Corollary}
\newtheorem{conjecture}[theorem]{Conjecture}

\theoremstyle{definition}
\newtheorem{definition}[theorem]{Definition}
\newtheorem{example}[theorem]{Example}
\newtheorem{exercise}[theorem]{Exercise}
\newtheorem{problem}[theorem]{Problem}
\newtheorem{question}[theorem]{Question}

\theoremstyle{remark}
\newtheorem*{remark}{Remark}
\newtheorem*{note}{Note}
\newtheorem*{solution}{Solution}



%Inequalities
\newcommand{\cycsum}{\sum_{\mathrm{cyc}}}
\newcommand{\symsum}{\sum_{\mathrm{sym}}}
\newcommand{\cycprod}{\prod_{\mathrm{cyc}}}
\newcommand{\symprod}{\prod_{\mathrm{sym}}}

%Linear Algebra

\DeclareMathOperator{\Span}{span}
\DeclareMathOperator{\im}{im}
\DeclareMathOperator{\diag}{diag}
\DeclareMathOperator{\Ker}{Ker}
\DeclareMathOperator{\ob}{ob}
\DeclareMathOperator{\Hom}{Hom}
\DeclareMathOperator{\Mor}{Mor}
\DeclareMathOperator{\sk}{sk}
\DeclareMathOperator{\Vect}{Vect}
\DeclareMathOperator{\Set}{Set}
\DeclareMathOperator{\Group}{Group}
\DeclareMathOperator{\Ring}{Ring}
\DeclareMathOperator{\Ab}{Ab}
\DeclareMathOperator{\Top}{Top}
\DeclareMathOperator{\hTop}{hTop}
\DeclareMathOperator{\Htpy}{Htpy}
\DeclareMathOperator{\Cat}{Cat}
\DeclareMathOperator{\CAT}{CAT}
\DeclareMathOperator{\Cone}{Cone}
\DeclareMathOperator{\dom}{dom}
\DeclareMathOperator{\cod}{cod}
\DeclareMathOperator{\Aut}{Aut}
\DeclareMathOperator{\Mat}{Mat}
\DeclareMathOperator{\Fin}{Fin}
\DeclareMathOperator{\rel}{rel}
\DeclareMathOperator{\Int}{Int}
\DeclareMathOperator{\sgn}{sgn}
\DeclareMathOperator{\Homeo}{Homeo}
\DeclareMathOperator{\SHomeo}{SHomeo}
\DeclareMathOperator{\PSL}{PSL}
\DeclareMathOperator{\Bil}{Bil}
\DeclareMathOperator{\Sym}{Sym}
\DeclareMathOperator{\Skew}{Skew}
\DeclareMathOperator{\Alt}{Alt}
\DeclareMathOperator{\Quad}{Quad}
\DeclareMathOperator{\Sin}{Sin}
\DeclareMathOperator{\Supp}{Supp}
\DeclareMathOperator{\Char}{char}
\DeclareMathOperator{\Teich}{Teich}
\DeclareMathOperator{\GL}{GL}
\DeclareMathOperator{\tr}{tr}
\DeclareMathOperator{\codim}{codim}
\DeclareMathOperator{\coker}{coker}
\DeclareMathOperator{\corank}{corank}
\DeclareMathOperator{\rank}{rank}
\DeclareMathOperator{\Diff}{Diff}
\DeclareMathOperator{\Bun}{Bun}
\DeclareMathOperator{\Sm}{Sm}
\DeclareMathOperator{\Fr}{Fr}
\DeclareMathOperator{\Cob}{Cob}
\DeclareMathOperator{\Ext}{Ext}
\DeclareMathOperator{\Tor}{Tor}



%Row operations
\newcommand{\elem}[1]{% elementary operations
\xrightarrow{\substack{#1}}%
}

\newcommand{\lelem}[1]{% elementary operations (left alignment)
\xrightarrow{\begin{subarray}{l}#1\end{subarray}}%
}

%SS
\DeclareMathOperator{\supp}{supp}
\DeclareMathOperator{\Var}{Var}

%NT
\DeclareMathOperator{\ord}{ord}

%Alg
\DeclareMathOperator{\Rad}{Rad}
\DeclareMathOperator{\Jac}{Jac}

%Misc
\newcommand{\SL}{{\mathrm{SL}}}
\newcommand{\mobgp}{{\mathrm{PSL}_2(\mathbb{C})}}
\newcommand{\id}{{\mathrm{id}}}
\newcommand{\MCG}{{\mathrm{MCG}}}
\newcommand{\PMCG}{{\mathrm{PMCG}}}
\newcommand{\SMCG}{{\mathrm{SMCG}}}
\newcommand{\ud}{{\mathrm{d}}}
\newcommand{\Vol}{{\mathrm{Vol}}}
\newcommand{\Area}{{\mathrm{Area}}}
\newcommand{\diam}{{\mathrm{diam}}}
\newcommand{\End}{{\mathrm{End}}}


\newcommand{\reg}{{\mathtt{reg}}}
\newcommand{\geo}{{\mathtt{geo}}}

\newcommand{\tori}{{\mathcal{T}}}
\newcommand{\cpn}{{\mathtt{c}}}
\newcommand{\pat}{{\mathtt{p}}}

\let\Cap\undefined
\newcommand{\Cap}{{\mathcal{C}}ap}
\newcommand{\Push}{{\mathcal{P}}ush}
\newcommand{\Forget}{{\mathcal{F}}orget}



\title{Assignment 1}
\author{Jonas Trepiakas}
\date{}

\renewcommand{\thesection}{\arabic{section}}

\begin{document}
\maketitle

\section{Problem 1}

    \begin{problem}[]
        Fix an isomorphism $H_n\left( S^{n} \right) \cong \mathbb{Z}$.
        We define the degree $\deg f$ of a map
        $f \colon S^{n} \to S^{n}$ to be the integer such that
        $f_* \colon H_n(S^{n}) \to H_n(S^{n})$ sends $1$ to
        $\deg f \in \mathbb{Z}$.
        \begin{enumerate}
            \item Show that taking the degree of a map
                $S^{n} \to S^{n}$ induces a well-defined
                map
                \[
                \deg \colon \pi_n(S^{n}) \to \mathbb{Z}
                \] 
            \item Show that $\deg $ is a group homomorphism.
            \item Show that the map $\deg$ is surjective.
            \item Suppose that $n\ge 2$. Show that
                $\pi_n\left( S^{n} \right) \cong
                \mathbb{Z} \times A$ for some abelian group $A$.
        \end{enumerate}
    \end{problem}

        \begin{proof}


        \begin{enumerate}
            \item Let
                $ \left[ f \right] 
                \in \pi_n \left( S^{n} \right) $ and
                suppose $f, f'$ are two representatives of
                this class. Then
                $f$ and $f'$ are homotopic by definition,
                so $f_* = \left( f' \right)_* \colon
                \mathbb{Z} = H_n\left( S^{n} \right) \to 
                H_n\left( S^{n} \right) = \mathbb{Z} $ are equal.
                In particular,
                $\deg f = f_*(1) = \left( f' \right)_* (1)
                = \deg f'$. So the map is well-defined.
            \item To show that degree is a group homomorphism,
                we must show that
                $\deg \left( f+g \right) = 
                \deg f + \deg g$.

                For this, we will show a couple of results.

                \begin{proposition}[]
                    Let $X = S_1^{n} \vee \ldots \vee
                    S_k^{n}$ for $n > 0$. Then
                    the homomorphism 
                    $H_n\left( S_1^{n} \right) \oplus \ldots
                    \oplus H_n\left( S_k^{n} \right) 
                    \to H_n(X)$ induced by the inclusion maps
                    is an isomorphism whose inverse
                    is induced by the projections
                    $X \to S_i^{n}$.
                \end{proposition}
                
                To prove this proposition, we must show the following
                lemma.

                \begin{lemma}[]
                    Let $X$ be a Hausdorff space and let
                    $x_0 \in X$ be a point having a closed
                    neighborhood $N$ in $X$ of which
                    $\left\{ x_0 \right\} $ is a strong deformation
                    retract. Let $Y$ be a Hausdorff space and
                    let $y_0 \in Y$. Define
                    $X \vee Y = X \times \left\{ y_0 \right\} 
                    \cup \left\{ x_0 \right\} \times Y$.
                    Then the inclusion maps induce
                    isomorphisms 
                    $\tilde{H}_i(X) \oplus \tilde{H}_i(Y)
                    \cong \tilde{H}_i\left( X \vee Y \right) $
                    whose inverse is induced by the projections
                    of $X \vee Y$ to $X$ and $Y$.
                \end{lemma}
                
                \begin{proof}[Proof of lemma]
                    Consider $A = X$ and
                    $U = X - N$ which is open, and
                    $\overline{U} \subset A$. Then by
                    excision,
                    $H_* \left( X \vee Y, X \right) 
                    \cong H_*\left( N \cup Y, N \right) 
                    \cong \tilde{H}_*\left( Y \right) $

                    Consider the LES of the triple
                    $\left( X \vee Y,
                    \left\{ x_0 \right\} \times Y,
                \left\{ x_0 \right\} \times 
            \left\{ y_0 \right\} \right) $. We obtain
            \[
            \ldots \to 
            H_p\left( \left\{ x_0 \right\} \times Y,
            \left( x_0,y_0 \right) \right)
            \stackrel{i_*}{\to}
            H_p\left( X \vee Y, \left( x_0,y_0 \right)  \right) 
            \stackrel{j_*}{\to} H_p\left( X \vee Y,
            \left\{ x_0 \right\} \times Y \right) \to \ldots
            \] 
            Since $\pi_Y \circ i = \id_{
            \left\{ x_0 \right\} \times Y} $, 
            $i_*$ is injective.

            Furthermore, we have
            \[
            H_p\left( X \vee Y, 
            \left( x_0, y_0 \right) \right) 
            \stackrel{\left( \pi_X \right)_* }{\to } 
            H_p \left( \left\{ x_0 \right\} \times Y,
            \left( x_0, y_0 \right) \right) 
            \cong H_p\left( X \vee Y , 
            \left\{ x_0 \right\} \times Y \right) 
            \] 
            so $j_* = \left( \pi_X \right)_*$ under these
            identifications, so, in particular, 
            $j_*$ is surjective. Therefore, our exact sequence
            is a SES:
            \[
            0 \to  H_p\left( Y, pt \right)
            \stackrel{i_*}{\to }
            H_p \left( X \vee Y, pt \right) 
            \stackrel{j_*}{\to }
            \underbrace{H_p \left( X \vee Y, Y \right)}_{
            \cong H_p\left( X, pt \right) } \to 0
            \] 
            It remains to show that this SES is split, but
            since
            $\pi_X \circ \iota_{X} = 
            \id_{\left\{ x_0 \right\} \times X}$,
            we have that $\iota_{X*}$ provides a section.

        \end{proof}

        \begin{proof}[Proof of proposition]
            This follows by induction on the lemma.
        \end{proof}

        Next, suppose that $E_1, \ldots, E_k$ are
        disjoint open subsets of $S^{n}$, each homeomorphic to
        $\mathbb{R}^{n}$ for $n>0$.
        Let $f \colon S^{n} \to Y$ be a map which takes
        $S^{n} - \bigcup E_i $ to $y_0$. Then
        $f$ factors through the quotient space
        $S^{n} / \left( S^{n} - \bigcup E_i  \right) 
        \cong S_1^{n} \vee \ldots \vee S_k^{n}$ where
        $S_i^{n} = S^{n} / \left( S^{n} - E_i \right) $:
        \[
            f \colon S^{n} \stackrel{g}{\to }
            S_1^{n} \vee \ldots \vee S_k^{n}
            \stackrel{h}{\to } Y
        \] 
        Let $\iota_{j} \colon S_j^{n} 
        \hookrightarrow S_1^{n} \vee \ldots \vee
        S_k^{n}$ be the $j$ th inclusion and let
        $p_j \colon S_1^{n} \vee \ldots \vee
        S_k^{n} \to S_j^{n}$ be the $j$ th projection.
        Then by the proposition,
        $\sum_j \iota_{j*} p_{j*} = \id_* \colon
        H_n \left( S_1^{n} \vee \ldots \vee S_k^{n} \right) 
        \to H_n \left( S_1^{n} \vee \ldots \vee
        S_k^{n}\right) $. Let
        $g_j = p_j \circ g \colon S^{n} \to S_j^{n}$ and
        $h_j = h \circ \iota_j \colon
        S_j^{n} \to Y$ and let
        $f_j = h_j \circ g_j \colon  S^{n} \to Y$.
        That is, $f_j$ is the map which is $f$ on
        $E_j$ and maps the complement of $E_j$ to the basepoint
        $y_0$.

        \begin{theorem}[]
            In the above situation, $f_*
            = \sum_{j=1}^{k} f_{j*} \colon
            H_n\left( S^{n} \right) \to H_n(Y)$.
        \end{theorem}

        \begin{proof}[Proof of theorem]
            We have
            $f_* = 
            h_* \circ g_* = 
            \sum_j h_* i_{j*} p_{j*} g_*
            = \sum_j h_{j*} g_{j*}
            = \sum_j f_{j*}$.
        \end{proof}

        Now we get back to showing that
        $\deg \left( f+g \right) = \deg f + \deg g$.

        Note that by way of defining
        $f+g$, this essentially maps $I^{n}$ by
        $f$ on the left half and $g$ on the right half with
        the boundary mapping to the base point $x_0$.
        In particular, this factors through the
        quotient $I^{n} \to I^{n} / \partial I^{n} 
        \cong S^{n}$, where now the two halves can be interpreted
        as, say, the upper and lower hemispheres. In particular,
        the equator is by assumption also mapped to
        $x_0$, so we can quotient further by
        $S^{n} \to S^{n} \vee S^{n}$ by "pinching" the equator
        to a point. This is essentially what the proposition
        above describes. In particular, $f+g$ can be covered
        by the two open hemispheres and maps the equator
        to $x_0$, so by the theorem,
        we have $\left( f+g \right)_*
        = f_* + g_*$, i.e.,
        $\deg (f+g) = \left( f+g \right)_*(1)
        = f_*(1) + g_*(1) = \deg f + \deg g$, as we wanted
        to show.

    \item 
        Next we show that $\deg$ is surjective. 
        First note that
        $\deg \id = \id_* (1) = 1$ by functoriality since
        $\id_* = \id_{H_n(S^{n})}$.
        By functoriality, we thus hit
        all of $\mathbb{Z}$. More precisely,
        $\deg \left( \ast_{n} \id \right) = n$ for
        $n \in \mathbb{N} $ as
        $\deg$ is a homomorphism.
        Also $\deg \left( \ast_{n} (-\id) \right) 
        = -n$ for $n \in \mathbb{N} $ and
        $\deg (c_{x_0}) = 0$, so
        $\deg$ is surjective.
    \item Let $n\ge 2$. We have a SES
        \[
        0 \to \ker \deg \to 
        \pi_n\left( S^{n} \right) \stackrel{\deg}{\to }
        \mathbb{Z} \to 0.
        \] 
        Since $\mathbb{Z}$ is projective, 
        this splits, so
        $\pi_n\left( S^{n} \right) 
        \cong \mathbb{Z} \oplus \ker \deg$.
        But $\ker \deg$ is a subgroup of
        $\pi_n\left( S^{n} \right) $ which is abelian, hence
        is itself abelian.







        \end{enumerate}

    \end{proof}

    \section{Problem 2}

    \begin{problem}[]
        Fix $n\ge 1$. We say that a space $X$ is
        \textit{$n$-connected} if it is non-empty, path-connected,
        and $\pi_k (X, x) = 0$ for all $1 \le k \le n$ and
        $x \in X$.
        For $\left( X, x_0 \right) $ a pointed, path-connected space,
        show that the following are equivalent:
        \begin{enumerate}
            \item $X$ is $n$-connected.
            \item $\pi_k\left( X,x_0 \right) = 0$ for all
                $1 \le k \le n$.
            \item Every map
                $S^{k} \to X$ can be extended to a map
                $D^{k+1} \to X$ for all $k \le n$.
            \item Every map
                $S^{k} \to X$ is homotopic to a constant
                map for all
                $k \le n$.
        \end{enumerate}
    \end{problem}

    \begin{proof}
        $\left( 1 \implies 2 \right) $: this follows since
        $X$ being $n$-connected means that $\pi_k\left( X,x \right) 
        = 0$ for all $x \in X$ and all $1\le k\le n$,
        hence in particular for $x_0$.\\
        $(2 \implies 3)$ : Let
        $f \colon S^{k} \to X$ be a map. 
        Then $f$ represents some homotopy class
        $\left[ f \right] \in \pi_k\left( X,x_0 \right) $. But
        since $\pi_k(X,x_0) = 0$, $f$ is homotopic to
        the constant map at $x_0 \rel s_0$.
        Let $H \colon S^{k} \times I \to X$ be this homotopy.
        Define
        $\tilde{f} \colon D^{k+1} \to X$ by
        $\tilde{f}(x) = H \left( x, \|x\| \right) $.
        Then $\tilde{f}$ is continuous as a composite of
        continuous maps and
        $\tilde{f}|_{S^{k}}(-) = 
        H\left( - , 1 \right) =
        f(-)$, so $\tilde{f}$ indeed extends $f$.\\
        $(3 \implies 4)$ : Let $f \colon S^{k} \to X$ be
        a map. Extends $f$ to a map
        $\tilde{f} \colon D^{k+1} \to X$. Define now
        a homotopy
        $H \colon S^{k} \times I \to X$ by
        $H\left( x,t \right) =
        \tilde{f}\left( xt \right) $. This is continuous
        and $H\left( x,1 \right) =
        \tilde{f}(x) = f(x)$ while
        $H\left( x,0 \right) = 
        \tilde{f}(0) \in X$ is constant. Hence this gives
        a homotopy between $f$ and $c_{\tilde{f}(0)}$.\\
        \linebreak
        $(4 \implies 3)$ : 
        Let $f \colon S^{k} \to X$ be a given map.
        By assumption, there exists
        a homotopy
        $H \colon S^{k} \times I \to X$ such that
        $H\left( -,1 \right) = f(-)$ and
        $H(-,0) = c$ where $c$ is some constant map
        at a point in $X$.
        But then $H$ factors through the quotient
        \begin{equation*}
        \begin{tikzcd}
            S^{k} \times I \ar[d] \ar[dr, "H"] & \\
            D^{k+1} \ar[r, "\tilde{H}"'] & X
        \end{tikzcd}
        \end{equation*}
        where we identify
        $S^{k} \times \left\{ 0 \right\} $ to a point.
        But then $\tilde{H}|_{S^{k}} (-) = 
        H\left( -, 1 \right) =
        f(-)$, so $\tilde{H}$ extends $f$.\\
        \linebreak
        $(3 \implies 2)$ : 
        Let $\left[ f \right] \in \pi_k(X, x_0)$ and
        $f$ a representative. 
        We want to show that $f$ is homotopic to the
        constant map at $x_0$ relative $\partial I^{k}$.
        We can consider $f$ as a map
        $\left( I^{k}, \partial I^{k} \right) \to 
        \left( X, x_0 \right) $.  
        Then suppose that we construct a homotopy
        $H \colon I^{k} \times I \to X$ as follows.
        At time $t$ we shrink the unit cube $I^{k}$ to
        $t$ times its size (so at $t= 1$, we simply have
        the normal unit cube, and at $t= 0$, we have
        no cube). Then inside the shrunken cube, we
        apply $f$ and outside the inner cube, we map everything
        to $x_0$. This gives a continuous homotopy
        from the constant map at $x_0$ at time $t=0$ to
        $f$ at time $t = 1$. Furthermore, it maps
        the boundary to $x_0$ at all times. Thus
        this gives the desired homotopy, so
        $\pi_k (X, x_0) = 0$ for all $1 \le k \le n$.\\
        \linebreak
        $\left( 2 \implies 1 \right) $ : the only thing that
        requires showing is that
        given that $\pi_k(X, x_0) = 0$ for all $k$, we then
        have $\pi_k \left( X, x \right) = 0$ for all $k$ and
        all $x \in X$. But this is precisely what the given
        hint says we are allowed to assume since
        $X$ is path connected. So we are done.
    \end{proof}





    %\printbibliography
\end{document}
